Updated Makefile; Moved more definitions to Smallstep_.v

common/Smallstep_.v
@@ -6,11 +6,451 @@ Require Import Events.
 Require Import Globalenvs.
 Require Import LanguageInterface_.
 Require Import Integers.
-Require Import Smallstep.
 Require Import AST.
 Require Import Values.
 
 Set Implicit Arguments.
+
+(** * Closures of transitions relations *)
+
+Section CLOSURES.
+
+  Variable genv: Type.
+  Variable state: Type.
+
+  (** A one-step transition relation has the following signature.
+  It is parameterized by a global environment, which does not
+  change during the transition.  It relates the initial state
+  of the transition with its final state.  The [trace] parameter
+  captures the observable events possibly generated during the
+  transition. *)
+
+  Variable step: genv -> state -> trace -> state -> Prop.
+
+  (** No transitions: stuck state *)
+
+  Definition nostep (ge: genv) (s: state) : Prop :=
+    forall t s', ~(step ge s t s').
+
+  (** Zero, one or several transitions.  Also known as Kleene closure,
+    or reflexive transitive closure. *)
+
+  Inductive star (ge: genv): state -> trace -> state -> Prop :=
+  | star_refl: forall s,
+      star ge s E0 s
+  | star_step: forall s1 t1 s2 t2 s3 t,
+      step ge s1 t1 s2 -> star ge s2 t2 s3 -> t = t1 ** t2 ->
+      star ge s1 t s3.
+
+  Lemma star_one:
+    forall ge s1 t s2, step ge s1 t s2 -> star ge s1 t s2.
+  Proof.
+    intros. eapply star_step; eauto. apply star_refl. traceEq.
+  Qed.
+
+  Lemma star_two:
+    forall ge s1 t1 s2 t2 s3 t,
+      step ge s1 t1 s2 -> step ge s2 t2 s3 -> t = t1 ** t2 ->
+      star ge s1 t s3.
+  Proof.
+    intros. eapply star_step; eauto. apply star_one; auto.
+  Qed.
+
+  Lemma star_three:
+    forall ge s1 t1 s2 t2 s3 t3 s4 t,
+      step ge s1 t1 s2 -> step ge s2 t2 s3 -> step ge s3 t3 s4 -> t = t1 ** t2 ** t3 ->
+      star ge s1 t s4.
+  Proof.
+    intros. eapply star_step; eauto. eapply star_two; eauto.
+  Qed.
+
+  Lemma star_four:
+    forall ge s1 t1 s2 t2 s3 t3 s4 t4 s5 t,
+      step ge s1 t1 s2 -> step ge s2 t2 s3 ->
+      step ge s3 t3 s4 -> step ge s4 t4 s5 -> t = t1 ** t2 ** t3 ** t4 ->
+      star ge s1 t s5.
+  Proof.
+    intros. eapply star_step; eauto. eapply star_three; eauto.
+  Qed.
+
+  Lemma star_trans:
+    forall ge s1 t1 s2, star ge s1 t1 s2 ->
+                   forall t2 s3 t, star ge s2 t2 s3 -> t = t1 ** t2 -> star ge s1 t s3.
+  Proof.
+    induction 1; intros.
+    rewrite H0. simpl. auto.
+    eapply star_step; eauto. traceEq.
+  Qed.
+
+  Lemma star_left:
+    forall ge s1 t1 s2 t2 s3 t,
+      step ge s1 t1 s2 -> star ge s2 t2 s3 -> t = t1 ** t2 ->
+      star ge s1 t s3.
+  Proof star_step.
+
+  Lemma star_right:
+    forall ge s1 t1 s2 t2 s3 t,
+      star ge s1 t1 s2 -> step ge s2 t2 s3 -> t = t1 ** t2 ->
+      star ge s1 t s3.
+  Proof.
+    intros. eapply star_trans. eauto. apply star_one. eauto. auto.
+  Qed.
+
+  Lemma star_E0_ind:
+    forall ge (P: state -> state -> Prop),
+      (forall s, P s s) ->
+      (forall s1 s2 s3, step ge s1 E0 s2 -> P s2 s3 -> P s1 s3) ->
+      forall s1 s2, star ge s1 E0 s2 -> P s1 s2.
+  Proof.
+    intros ge P BASE REC.
+    assert (forall s1 t s2, star ge s1 t s2 -> t = E0 -> P s1 s2).
+    induction 1; intros; subst.
+    auto.
+    destruct (Eapp_E0_inv _ _ H2). subst. eauto.
+    eauto.
+  Qed.
+
+  (** One or several transitions.  Also known as the transitive closure. *)
+
+  Inductive plus (ge: genv): state -> trace -> state -> Prop :=
+  | plus_left: forall s1 t1 s2 t2 s3 t,
+      step ge s1 t1 s2 -> star ge s2 t2 s3 -> t = t1 ** t2 ->
+      plus ge s1 t s3.
+
+  Lemma plus_one:
+    forall ge s1 t s2,
+      step ge s1 t s2 -> plus ge s1 t s2.
+  Proof.
+    intros. econstructor; eauto. apply star_refl. traceEq.
+  Qed.
+
+  Lemma plus_two:
+    forall ge s1 t1 s2 t2 s3 t,
+      step ge s1 t1 s2 -> step ge s2 t2 s3 -> t = t1 ** t2 ->
+      plus ge s1 t s3.
+  Proof.
+    intros. eapply plus_left; eauto. apply star_one; auto.
+  Qed.
+
+  Lemma plus_three:
+    forall ge s1 t1 s2 t2 s3 t3 s4 t,
+      step ge s1 t1 s2 -> step ge s2 t2 s3 -> step ge s3 t3 s4 -> t = t1 ** t2 ** t3 ->
+      plus ge s1 t s4.
+  Proof.
+    intros. eapply plus_left; eauto. eapply star_two; eauto.
+  Qed.
+
+  Lemma plus_four:
+    forall ge s1 t1 s2 t2 s3 t3 s4 t4 s5 t,
+      step ge s1 t1 s2 -> step ge s2 t2 s3 ->
+      step ge s3 t3 s4 -> step ge s4 t4 s5 -> t = t1 ** t2 ** t3 ** t4 ->
+      plus ge s1 t s5.
+  Proof.
+    intros. eapply plus_left; eauto. eapply star_three; eauto.
+  Qed.
+
+  Lemma plus_star:
+    forall ge s1 t s2, plus ge s1 t s2 -> star ge s1 t s2.
+  Proof.
+    intros. inversion H; subst.
+    eapply star_step; eauto.
+  Qed.
+
+  Lemma plus_right:
+    forall ge s1 t1 s2 t2 s3 t,
+      star ge s1 t1 s2 -> step ge s2 t2 s3 -> t = t1 ** t2 ->
+      plus ge s1 t s3.
+  Proof.
+    intros. inversion H; subst. simpl. apply plus_one. auto.
+    rewrite Eapp_assoc. eapply plus_left; eauto.
+    eapply star_right; eauto.
+  Qed.
+
+  Lemma plus_left':
+    forall ge s1 t1 s2 t2 s3 t,
+      step ge s1 t1 s2 -> plus ge s2 t2 s3 -> t = t1 ** t2 ->
+      plus ge s1 t s3.
+  Proof.
+    intros. eapply plus_left; eauto. apply plus_star; auto.
+  Qed.
+
+  Lemma plus_right':
+    forall ge s1 t1 s2 t2 s3 t,
+      plus ge s1 t1 s2 -> step ge s2 t2 s3 -> t = t1 ** t2 ->
+      plus ge s1 t s3.
+  Proof.
+    intros. eapply plus_right; eauto. apply plus_star; auto.
+  Qed.
+
+  Lemma plus_star_trans:
+    forall ge s1 t1 s2 t2 s3 t,
+      plus ge s1 t1 s2 -> star ge s2 t2 s3 -> t = t1 ** t2 -> plus ge s1 t s3.
+  Proof.
+    intros. inversion H; subst.
+    econstructor; eauto. eapply star_trans; eauto.
+    traceEq.
+  Qed.
+
+  Lemma star_plus_trans:
+    forall ge s1 t1 s2 t2 s3 t,
+      star ge s1 t1 s2 -> plus ge s2 t2 s3 -> t = t1 ** t2 -> plus ge s1 t s3.
+  Proof.
+    intros. inversion H; subst.
+    simpl; auto.
+    rewrite Eapp_assoc.
+    econstructor. eauto. eapply star_trans. eauto.
+    apply plus_star. eauto. eauto. auto.
+  Qed.
+
+  Lemma plus_trans:
+    forall ge s1 t1 s2 t2 s3 t,
+      plus ge s1 t1 s2 -> plus ge s2 t2 s3 -> t = t1 ** t2 -> plus ge s1 t s3.
+  Proof.
+    intros. eapply plus_star_trans. eauto. apply plus_star. eauto. auto.
+  Qed.
+
+  Lemma plus_inv:
+    forall ge s1 t s2,
+      plus ge s1 t s2 ->
+      step ge s1 t s2 \/ exists s', exists t1, exists t2, step ge s1 t1 s' /\ plus ge s' t2 s2 /\ t = t1 ** t2.
+  Proof.
+    intros. inversion H; subst. inversion H1; subst.
+    left. rewrite E0_right. auto.
+    right. exists s3; exists t1; exists (t0 ** t3); split. auto.
+    split. econstructor; eauto. auto.
+  Qed.
+
+  Lemma star_inv:
+    forall ge s1 t s2,
+      star ge s1 t s2 ->
+      (s2 = s1 /\ t = E0) \/ plus ge s1 t s2.
+  Proof.
+    intros. inv H. left; auto. right; econstructor; eauto.
+  Qed.
+
+  Lemma plus_ind2:
+    forall ge (P: state -> trace -> state -> Prop),
+      (forall s1 t s2, step ge s1 t s2 -> P s1 t s2) ->
+      (forall s1 t1 s2 t2 s3 t,
+          step ge s1 t1 s2 -> plus ge s2 t2 s3 -> P s2 t2 s3 -> t = t1 ** t2 ->
+          P s1 t s3) ->
+      forall s1 t s2, plus ge s1 t s2 -> P s1 t s2.
+  Proof.
+    intros ge P BASE IND.
+    assert (forall s1 t s2, star ge s1 t s2 ->
+                       forall s0 t0, step ge s0 t0 s1 ->
+                                P s0 (t0 ** t) s2).
+    induction 1; intros.
+    rewrite E0_right. apply BASE; auto.
+    eapply IND. eauto. econstructor; eauto. subst t. eapply IHstar; eauto. auto.
+
+    intros. inv H0. eauto.
+  Qed.
+
+  Lemma plus_E0_ind:
+    forall ge (P: state -> state -> Prop),
+      (forall s1 s2 s3, step ge s1 E0 s2 -> star ge s2 E0 s3 -> P s1 s3) ->
+      forall s1 s2, plus ge s1 E0 s2 -> P s1 s2.
+  Proof.
+    intros. inv H0. exploit Eapp_E0_inv; eauto. intros [A B]; subst. eauto.
+  Qed.
+
+  (** Counted sequences of transitions *)
+
+  Inductive starN (ge: genv): nat -> state -> trace -> state -> Prop :=
+  | starN_refl: forall s,
+      starN ge O s E0 s
+  | starN_step: forall n s t t1 s' t2 s'',
+      step ge s t1 s' -> starN ge n s' t2 s'' -> t = t1 ** t2 ->
+      starN ge (S n) s t s''.
+
+  Remark starN_star:
+    forall ge n s t s', starN ge n s t s' -> star ge s t s'.
+  Proof.
+    induction 1; econstructor; eauto.
+  Qed.
+
+  Remark star_starN:
+    forall ge s t s', star ge s t s' -> exists n, starN ge n s t s'.
+  Proof.
+    induction 1.
+    exists O; constructor.
+    destruct IHstar as [n P]. exists (S n); econstructor; eauto.
+  Qed.
+
+  (** Infinitely many transitions *)
+
+  CoInductive forever (ge: genv): state -> traceinf -> Prop :=
+  | forever_intro: forall s1 t s2 T,
+      step ge s1 t s2 -> forever ge s2 T ->
+      forever ge s1 (t *** T).
+
+  Lemma star_forever:
+    forall ge s1 t s2, star ge s1 t s2 ->
+                  forall T, forever ge s2 T ->
+                       forever ge s1 (t *** T).
+  Proof.
+    induction 1; intros. simpl. auto.
+    subst t. rewrite Eappinf_assoc.
+    econstructor; eauto.
+  Qed.
+
+  (** An alternate, equivalent definition of [forever] that is useful
+    for coinductive reasoning. *)
+
+  Variable A: Type.
+  Variable order: A -> A -> Prop.
+
+  CoInductive forever_N (ge: genv) : A -> state -> traceinf -> Prop :=
+  | forever_N_star: forall s1 t s2 a1 a2 T1 T2,
+      star ge s1 t s2 ->
+      order a2 a1 ->
+      forever_N ge a2 s2 T2 ->
+      T1 = t *** T2 ->
+      forever_N ge a1 s1 T1
+  | forever_N_plus: forall s1 t s2 a1 a2 T1 T2,
+      plus ge s1 t s2 ->
+      forever_N ge a2 s2 T2 ->
+      T1 = t *** T2 ->
+      forever_N ge a1 s1 T1.
+
+  Hypothesis order_wf: well_founded order.
+
+  Lemma forever_N_inv:
+    forall ge a s T,
+      forever_N ge a s T ->
+      exists t, exists s', exists a', exists T',
+              step ge s t s' /\ forever_N ge a' s' T' /\ T = t *** T'.
+  Proof.
+    intros ge a0. pattern a0. apply (well_founded_ind order_wf).
+    intros. inv H0.
+    (* star case *)
+    inv H1.
+    (* no transition *)
+    change (E0 *** T2) with T2. apply H with a2. auto. auto.
+    (* at least one transition *)
+    exists t1; exists s0; exists x; exists (t2 *** T2).
+    split. auto. split. eapply forever_N_star; eauto.
+    apply Eappinf_assoc.
+    (* plus case *)
+    inv H1.
+    exists t1; exists s0; exists a2; exists (t2 *** T2).
+    split. auto.
+    split. inv H3. auto.
+    eapply forever_N_plus. econstructor; eauto. eauto. auto.
+    apply Eappinf_assoc.
+  Qed.
+
+  Lemma forever_N_forever:
+    forall ge a s T, forever_N ge a s T -> forever ge s T.
+  Proof.
+    cofix COINDHYP; intros.
+    destruct (forever_N_inv H) as [t [s' [a' [T' [P [Q R]]]]]].
+    rewrite R. apply forever_intro with s'. auto.
+    apply COINDHYP with a'; auto.
+  Qed.
+
+  (** Yet another alternative definition of [forever]. *)
+
+  CoInductive forever_plus (ge: genv) : state -> traceinf -> Prop :=
+  | forever_plus_intro: forall s1 t s2 T1 T2,
+      plus ge s1 t s2 ->
+      forever_plus ge s2 T2 ->
+      T1 = t *** T2 ->
+      forever_plus ge s1 T1.
+
+  Lemma forever_plus_inv:
+    forall ge s T,
+      forever_plus ge s T ->
+      exists s', exists t, exists T',
+            step ge s t s' /\ forever_plus ge s' T' /\ T = t *** T'.
+  Proof.
+    intros. inv H. inv H0. exists s0; exists t1; exists (t2 *** T2).
+    split. auto.
+    split. exploit star_inv; eauto. intros [[P Q] | R].
+    subst. simpl. auto. econstructor; eauto.
+    traceEq.
+  Qed.
+
+  Lemma forever_plus_forever:
+    forall ge s T, forever_plus ge s T -> forever ge s T.
+  Proof.
+    cofix COINDHYP; intros.
+    destruct (forever_plus_inv H) as [s' [t [T' [P [Q R]]]]].
+    subst. econstructor; eauto.
+  Qed.
+
+  (** Infinitely many silent transitions *)
+
+  CoInductive forever_silent (ge: genv): state -> Prop :=
+  | forever_silent_intro: forall s1 s2,
+      step ge s1 E0 s2 -> forever_silent ge s2 ->
+      forever_silent ge s1.
+
+  (** An alternate definition. *)
+
+  CoInductive forever_silent_N (ge: genv) : A -> state -> Prop :=
+  | forever_silent_N_star: forall s1 s2 a1 a2,
+      star ge s1 E0 s2 ->
+      order a2 a1 ->
+      forever_silent_N ge a2 s2 ->
+      forever_silent_N ge a1 s1
+  | forever_silent_N_plus: forall s1 s2 a1 a2,
+      plus ge s1 E0 s2 ->
+      forever_silent_N ge a2 s2 ->
+      forever_silent_N ge a1 s1.
+
+  Lemma forever_silent_N_inv:
+    forall ge a s,
+      forever_silent_N ge a s ->
+      exists s', exists a',
+          step ge s E0 s' /\ forever_silent_N ge a' s'.
+  Proof.
+    intros ge a0. pattern a0. apply (well_founded_ind order_wf).
+    intros. inv H0.
+    (* star case *)
+    inv H1.
+    (* no transition *)
+    apply H with a2. auto. auto.
+    (* at least one transition *)
+    exploit Eapp_E0_inv; eauto. intros [P Q]. subst.
+    exists s0; exists x.
+    split. auto. eapply forever_silent_N_star; eauto.
+    (* plus case *)
+    inv H1. exploit Eapp_E0_inv; eauto. intros [P Q]. subst.
+    exists s0; exists a2.
+    split. auto. inv H3. auto.
+    eapply forever_silent_N_plus. econstructor; eauto. eauto.
+  Qed.
+
+  Lemma forever_silent_N_forever:
+    forall ge a s, forever_silent_N ge a s -> forever_silent ge s.
+  Proof.
+    cofix COINDHYP; intros.
+    destruct (forever_silent_N_inv H) as [s' [a' [P Q]]].
+    apply forever_silent_intro with s'. auto.
+    apply COINDHYP with a'; auto.
+  Qed.
+
+  (** Infinitely many non-silent transitions *)
+
+  CoInductive forever_reactive (ge: genv): state -> traceinf -> Prop :=
+  | forever_reactive_intro: forall s1 s2 t T,
+      star ge s1 t s2 -> t <> E0 -> forever_reactive ge s2 T ->
+      forever_reactive ge s1 (t *** T).
+
+  Lemma star_forever_reactive:
+    forall ge s1 t s2 T,
+      star ge s1 t s2 -> forever_reactive ge s2 T ->
+      forever_reactive ge s1 (t *** T).
+  Proof.
+    intros. inv H0. rewrite <- Eappinf_assoc. econstructor.
+    eapply star_trans; eauto.
+    red; intro. exploit Eapp_E0_inv; eauto. intros [P Q]. contradiction.
+    auto.
+  Qed.
+
+End CLOSURES.
 
 (* The footprint of a concrete program is the set of identifiers that correspond
    to internal function definitions. The calls to these functions are not
@@ -117,6 +557,8 @@ Notation " 'Forever_silent' L p " := (forever_silent (step L p) (globalenv L)) (
 Notation " 'Forever_reactive' L p " := (forever_reactive (step L p) (globalenv L)) (at level 1, L at level 1) : smallstep_scope.
 Notation " 'Nostep' L p " := (nostep (step L p) (globalenv L)) (at level 1, L at level 1) : smallstep_scope.
 
+Open Scope smallstep_scope.
+
 Notation Semantics_gen step initial_state at_ext after_ext final_state globalenv p :=
   {|
   skel := AST.erase_program p;
@@ -166,6 +608,27 @@ Section FSIM.
   }.
 
 Arguments fsim_properties : clear implicits.
+
+(** An alternate form of the simulation diagram *)
+
+Lemma fsim_simulation':
+  forall L1 L2 index order match_states, fsim_properties L1 L2 index order match_states ->
+  forall i s1 t s1', Step L1 qset s1 t s1' ->
+  forall s2, match_states i s1 s2 ->
+  (exists i', exists s2', Plus L2 qset s2 t s2' /\ match_states i' s1' s2')
+  \/ (exists i', order i' i /\ t = E0 /\ match_states i' s1' s2).
+Proof.
+  intros. exploit @fsim_simulation; eauto.
+  intros [i' [s2' [A B]]]. intuition.
+  left; exists i'; exists s2'; auto.
+  inv H3.
+  right; exists i'; auto.
+  left; exists i'; exists s2'; split; auto. econstructor; eauto.
+Qed.
+
+(** ** Forward simulation diagrams. *)
+
+(** Various simulation diagrams that imply forward simulation *)
 
 Section FORWARD_SIMU_DIAGRAMS.
 
@@ -281,6 +744,49 @@ End SIMULATION_STEP.
 
 End FORWARD_SIMU_DIAGRAMS.
 
+(** ** Forward simulation of transition sequences *)
+
+Section SIMULATION_SEQUENCES.
+
+Context L1 L2 index order match_states (S: fsim_properties L1 L2 index order match_states).
+
+Lemma simulation_star:
+  forall s1 t s1', Star L1 qset s1 t s1' ->
+  forall i s2, match_states i s1 s2 ->
+  exists i', exists s2', Star L2 qset s2 t s2' /\ match_states i' s1' s2'.
+Proof.
+  induction 1; intros.
+  exists i; exists s2; split; auto. apply star_refl.
+  exploit fsim_simulation; eauto. intros [i' [s2' [A B]]].
+  exploit IHstar; eauto. intros [i'' [s2'' [C D]]].
+  exists i''; exists s2''; split; auto. eapply star_trans; eauto.
+  intuition auto. apply plus_star; auto.
+Qed.
+
+Lemma simulation_plus:
+  forall s1 t s1', Plus L1 qset s1 t s1' ->
+  forall i s2, match_states i s1 s2 ->
+  (exists i', exists s2', Plus L2 qset s2 t s2' /\ match_states i' s1' s2')
+  \/ (exists i', clos_trans _ order i' i /\ t = E0 /\ match_states i' s1' s2).
+Proof.
+  induction 1 using plus_ind2; intros.
+(* base case *)
+  exploit fsim_simulation'; eauto. intros [A | [i' A]].
+  left; auto.
+  right; exists i'; intuition.
+(* inductive case *)
+  exploit fsim_simulation'; eauto. intros [[i' [s2' [A B]]] | [i' [A [B C]]]].
+  exploit simulation_star. apply plus_star; eauto. eauto.
+  intros [i'' [s2'' [P Q]]].
+  left; exists i''; exists s2''; split; auto. eapply plus_star_trans; eauto.
+  exploit IHplus; eauto. intros [[i'' [s2'' [P Q]]] | [i'' [P [Q R]]]].
+  subst. simpl. left; exists i''; exists s2''; auto.
+  subst. simpl. right; exists i''; intuition auto.
+  eapply t_trans; eauto. eapply t_step; eauto.
+Qed.
+
+End SIMULATION_SEQUENCES.
+
 End FSIM.
 
 Arguments fsim_properties {_ _} _ {_ _} _ _ _ _ {_ _} _ L1 L2 index order match_states.
@@ -329,6 +835,107 @@ Proof.
     + erewrite fsim_footprint; eauto.
     + erewrite match_senv_symbol_address; eauto.
 Qed.
+
+(** ** Identity simulation *)
+
+Definition identity_fsim_components {liA liB} (L: semantics liA liB):
+  fsim_components cc_id cc_id L L.
+Proof.
+  eapply Forward_simulation with _ (fun _ _ _ => _); auto.
+  - firstorder.
+  - intros se _ [ ] qset [ ] _.
+    eapply forward_simulation_plus with (match_states := eq);
+    cbn; intros; subst; eauto 10 using plus_one.
+    exists tt, q1. intuition (subst; eauto).
+  - apply well_founded_ltof.
+Qed.
+
+Lemma identity_forward_simulation {liA liB} (L: semantics liA liB):
+  forward_simulation cc_id cc_id L L.
+Proof.
+  constructor. apply identity_fsim_components.
+Qed.
+
+(** ** Composing two forward simulations *)
+
+Section COMPOSE_FORWARD_SIMULATIONS.
+
+Context {liA1 liA2 liA3} {ccA12: callconv liA1 liA2} {ccA23: callconv liA2 liA3}.
+Context {liB1 liB2 liB3} {ccB12: callconv liB1 liB2} {ccB23: callconv liB2 liB3}.
+Context (L1: semantics liA1 liB1) (L2: semantics liA2 liB2) (L3: semantics liA3 liB3).
+
+Lemma compose_fsim_components:
+  fsim_components ccA12 ccB12 L1 L2 ->
+  fsim_components ccA23 ccB23 L2 L3 ->
+  fsim_components (ccA12 @ ccA23) (ccB12 @ ccB23) L1 L3.
+Proof.
+  intros [index order match_states Hsk props order_wf].
+  intros [index' order' match_states' Hsk' props' order_wf'].
+  set (ff_index := (index' * index)%type).
+  set (ff_order := lex_ord (clos_trans _ order') order).
+  set (ff_match_states :=
+         fun se1 se3 '(se2, w, w') (i: ff_index) (s1: state L1) (s3: state L3) =>
+           exists s2,
+             match_states se1 se2 w (snd i) s1 s2 /\
+             match_states' se2 se3 w' (fst i) s2 s3).
+  apply Forward_simulation with ff_order ff_match_states.
+  4: { unfold ff_order. auto using wf_lex_ord, wf_clos_trans. }
+  1: { congruence. }
+  1: { firstorder. }
+  intros se1 se3 [[se2 w] w'] qset (Hse12 & Hse23) Hse1. cbn in *.
+  assert (Hse2: Genv.valid_for (skel L2) se2).
+  { rewrite <- Hsk. eapply match_senv_valid_for; eauto. }
+  constructor.
+(* - (* valid query *) *)
+(*   intros q1 q3 (q2 & Hq12 & Hq23). *)
+(*   erewrite fsim_match_valid_query by eauto. *)
+(*   eapply fsim_match_valid_query; eauto. *)
+- (* initial states *)
+  intros q1 q3 s1 (q2 & Hq12 & Hq23) Hs1.
+  edestruct (@fsim_match_initial_states liA1) as (i & s2 & A & B); eauto.
+  edestruct (@fsim_match_initial_states liA2) as (i' & s3 & C & D); eauto.
+  exists (i', i); exists s3; split; auto. exists s2; auto.
+- (* final states *)
+  intros. cbn. destruct H as (s3 & A & B).
+  edestruct (@fsim_match_final_states liA1) as (r2 & Hr2 & Hr12); eauto.
+  edestruct (@fsim_match_final_states liA2) as (r3 & Hr3 & Hr23); eauto.
+- (* external states *)
+  intros. destruct H as [s3 [A B]].
+  edestruct (@fsim_match_external liA1) as (w12 & q2 & Hq2 & Hq12 & Hw12 & Hk12); eauto.
+  edestruct (@fsim_match_external liA2) as (w23 & q3 & Hq3 & Hq23 & Hw23 & Hk23); eauto.
+  exists (se2, w12, w23), q3. cbn; repeat apply conj; eauto.
+  intros r1 r3 s1' (r2 & Hr12 & Hr23) Hs1'.
+  edestruct Hk12 as (i12' & s2' & Hs2' & Hs12'); eauto.
+  edestruct Hk23 as (i23' & s3' & Hs3' & Hs23'); eauto.
+  exists (i23', i12'), s3'. split; auto. exists s2'; auto.
+- (* simulation *)
+  intros. destruct H0 as [s3 [A B]]. destruct i as [i2 i1]; simpl in *.
+  edestruct (@fsim_simulation' liA1) as [(i1' & s3' & C & D) | (i1' & C & D & E)]; eauto.
++ (* L2 makes one or several steps. *)
+  edestruct (@simulation_plus liA2) as [(i2' & s2' & P & Q) | (i2' & P & Q & R)]; eauto.
+* (* L3 makes one or several steps *)
+  exists (i2', i1'); exists s2'; split. auto. exists s3'; auto.
+* (* L3 makes no step *)
+  exists (i2', i1'); exists s2; split.
+  right; split. subst t; apply star_refl. red. left. auto.
+  exists s3'; auto.
++ (* L2 makes no step *)
+  exists (i2, i1'); exists s2; split.
+  right; split. subst t; apply star_refl. red. right. auto.
+  exists s3; auto.
+  Unshelve. auto. auto. auto. auto. auto. auto.
+Qed.
+
+Lemma compose_forward_simulations:
+  forward_simulation ccA12 ccB12 L1 L2 ->
+  forward_simulation ccA23 ccB23 L2 L3 ->
+  forward_simulation (ccA12 @ ccA23) (ccB12 @ ccB23) L1 L3.
+Proof.
+  intros [X] [Y]. constructor.
+  apply compose_fsim_components; auto.
+Qed.
+
+End COMPOSE_FORWARD_SIMULATIONS.
 
 (** * Receptiveness and determinacy *)
 
