common/CategoricalComp.v
@@ -5,11 +5,11 @@ Require Import LanguageInterface_.
 Require Import Events.
 Require Import Globalenvs.
 Require Import SmallstepLinking_.
-Require Import Smallstep.
 Require Import Smallstep_.
 Require Import Integers.
 Require Import Linking.
 Require Import AST.
+Require Import CallconvAlgebra_.
 
 Require Import Coq.Logic.ClassicalFacts.
 Require Import Coq.Logic.FunctionalExtensionality.
